src/aexp/properties.lean
@@ -11,12 +11,17 @@ namespace aexp -----------------------------------------------------------------
 
 variables {V : Type} [decidable_eq V] -- Type of variable names
 variables {vs : Type → Type} [vset vs V] -- Type of variable name sets
-variables {X : vs V} -- Variable name sets
+variables {X Y : vs V} -- Variable name sets
 
 -- Paper: Proposition 6.1 (b)
-theorem self_eq_subst_id_self (α : aexp X)
-: α = aexp.subst.apply (exp.subst.id X) α :=
-  quot.induction_on α $ λ e, quot.sound $ aeq.self_aeq_subst_id_self e
+theorem self_eq_subst_var_self (α : aexp X)
+: α = aexp.subst.apply exp.var α :=
+  quot.induction_on α $ λ e, quot.sound $ aeq.self_aeq_subst_var e
+
+-- Paper: Proposition 6.2
+theorem subst_F_comp_var_eq_F (F : exp.subst X Y) (x : ν∈ X)
+: aexp.subst.apply F (aexp.of_exp (exp.var x)) = aexp.of_exp (F x) :=
+  by apply quot.lift_beta (aexp.of_exp ∘ exp.subst.apply F) (eq_of_aeq_id F) (exp.var x)
 
 end /- namespace -/ aexp -------------------------------------------------------
 end /- namespace -/ acie -------------------------------------------------------
